Update recovery adequacy proof.

src/program_logic/recovery_adequacy.v
@@ -2,11 +2,11 @@ From iris.proofmode Require Import tactics.
 From iris.algebra Require Import gmap auth agree gset coPset.
 From iris.base_logic.lib Require Import wsat.
 From iris.program_logic Require Export weakestpre.
-From Perennial.program_logic Require Export crash_lang crash_weakestpre.
+From Perennial.program_logic Require Export staged_invariant crash_lang crash_weakestpre.
 Import uPred.
 
 Section crash_adequacy.
-Context `{!irisG Λ Σ}.
+Context `{!irisG Λ Σ, crashG Σ}.
 Implicit Types s : stuckness.
 Implicit Types k : nat.
 Implicit Types e : expr Λ.
@@ -18,43 +18,47 @@ Notation wptp s k t := ([∗ list] ef ∈ t, WPC ef @ s; k; ⊤; ∅ {{ fork_pos
 
 Lemma wpc_step s k e1 σ1 κ κs e2 σ2 efs m Φ Φc :
   prim_step e1 σ1 κ e2 σ2 efs →
-  state_interp σ1 (κ ++ κs) m -∗ WPC e1 @ s; k; ⊤; ∅ {{ Φ }} {{ Φc }} -∗
-  |={⊤,⊤}_(2 * (S (S k)))=>
+  state_interp σ1 (κ ++ κs) m -∗ WPC e1 @ s; k; ⊤; ∅ {{ Φ }} {{ Φc }} -∗ NC -∗
+  |={⊤,⊤}_(3 * (S (S k)))=>
   state_interp σ2 κs (length efs + m) ∗
   WPC e2 @ s; k; ⊤; ∅ {{ Φ }} {{ Φc }} ∗
-  wptp s k efs.
+  wptp s k efs ∗
+  NC.
 Proof.
-  rewrite {1}wpc_unfold /wpc_pre. iIntros (?) "Hσ H".
+  rewrite {1}wpc_unfold /wpc_pre. iIntros (?) "Hσ H HNC".
   rewrite (val_stuck e1 σ1 κ e2 σ2 efs) //.
   iDestruct "H" as "(H&_)".
-  replace (2 * S (S k)) with (S (S k) + S (S k)) by lia.
-  rewrite Nat_iter_add Nat_iter_S.
-  iMod ("H" $! σ1 with "Hσ") as "H".
+  replace (3 * S (S k)) with (S (S k) + S (S k) + S (S k)) by lia.
+  rewrite Nat_iter_add Nat_iter_add Nat_iter_S.
+  iMod ("H" $! σ1 with "Hσ HNC") as "H".
   do 4 iModIntro. iApply (step_fupdN_wand with "H").
   iIntros "H". rewrite Nat_iter_S.
   iMod "H" as "(_ & H)".
   iMod ("H" $! e2 σ2 efs with "[//]") as "H".
-  iIntros "!> !>". by iMod "H".
+  iIntros "!> !> !>".
+  iApply (step_fupdN_wand with "H"). iIntros "H".
+  iEval (rewrite Nat_iter_S). do 2 iMod "H". iModIntro. iNext.
+  by iMod "H".
 Qed.
 
 Lemma wptp_step s k e1 t1 t2 κ κs σ1 σ2 Φ Φc :
   step (e1 :: t1,σ1) κ (t2, σ2) →
-  state_interp σ1 (κ ++ κs) (length t1) -∗ WPC e1 @ s; k; ⊤; ∅ {{ Φ }} {{ Φc }}-∗ wptp s k t1 ==∗
+  state_interp σ1 (κ ++ κs) (length t1) -∗ WPC e1 @ s; k; ⊤; ∅ {{ Φ }} {{ Φc }}-∗ wptp s k t1 -∗ NC ==∗
   ∃ e2 t2', ⌜t2 = e2 :: t2'⌝ ∗
-  |={⊤,⊤}_(2 * (S (S k)))=> state_interp σ2 κs (pred (length t2)) ∗ WPC e2 @ s; k; ⊤; ∅ {{ Φ }} {{ Φc}} ∗ wptp s k t2'.
+  |={⊤,⊤}_(3 * (S (S k)))=> state_interp σ2 κs (pred (length t2)) ∗ WPC e2 @ s; k; ⊤; ∅ {{ Φ }} {{ Φc}} ∗ wptp s k t2' ∗ NC.
 Proof.
-  iIntros (Hstep) "Hσ He Ht".
+  iIntros (Hstep) "Hσ He Ht HNC".
   destruct Hstep as [e1' σ1' e2' σ2' efs [|? t1'] t2' ?? Hstep]; simplify_eq/=.
   - iExists e2', (t2' ++ efs). iModIntro. iSplitR; first by eauto.
-    iMod (wpc_step with "Hσ He") as "H"; first done.
+    iMod (wpc_step with "Hσ He HNC") as "H"; first done.
     iApply (step_fupdN_wand with "H"). iModIntro. iIntros "H".
-    iMod "H" as "(Hσ & He2 & Hefs)".
+    iMod "H" as "(Hσ & He2 & Hefs & HNC)".
     iIntros "!>". rewrite Nat.add_comm app_length. iFrame.
   - iExists e, (t1' ++ e2' :: t2' ++ efs); iSplitR; first eauto.
     iDestruct "Ht" as "(Ht1 & He1 & Ht2)".
-    iModIntro. iMod (wpc_step with "Hσ He1") as "H"; first done.
+    iModIntro. iMod (wpc_step with "Hσ He1 HNC") as "H"; first done.
     iApply (step_fupdN_wand with "H"). iModIntro. iIntros "H".
-    iMod "H" as "(Hσ & He2 & Hefs)". iIntros "!>".
+    iMod "H" as "(Hσ & He2 & Hefs & HNC)". iIntros "!>".
     iFrame "He". rewrite !app_length /= !app_length.
     replace (length t1' + S (length t2' + length efs))
       with (length efs + (length t1' + S (length t2'))) by omega. iFrame.
@@ -62,31 +66,32 @@ Qed.
 
 Lemma wptp_steps s k n e1 t1 κs κs' t2 σ1 σ2 Φ Φc :
   nsteps n (e1 :: t1, σ1) κs (t2, σ2) →
-  state_interp σ1 (κs ++ κs') (length t1) -∗ WPC e1 @ s; k; ⊤; ∅ {{ Φ }} {{ Φc }} -∗ wptp s k t1 -∗
-  |={⊤,⊤}_(2 * (S (S k)))=>^n (∃ e2 t2',
+  state_interp σ1 (κs ++ κs') (length t1) -∗ WPC e1 @ s; k; ⊤; ∅ {{ Φ }} {{ Φc }} -∗ wptp s k t1 -∗ NC -∗
+  |={⊤,⊤}_(3 * (S (S k)))=>^n (∃ e2 t2',
     ⌜t2 = e2 :: t2'⌝ ∗
     state_interp σ2 κs' (pred (length t2)) ∗
-    WPC e2 @ s; k; ⊤; ∅ {{ Φ }} {{ Φc }} ∗ wptp s k t2').
+    WPC e2 @ s; k; ⊤; ∅ {{ Φ }} {{ Φc }} ∗ wptp s k t2' ∗
+    NC).
 Proof.
   revert e1 t1 κs κs' t2 σ1 σ2; simpl.
   induction n as [|n IH]=> e1 t1 κs κs' t2 σ1 σ2 /=.
-  { inversion_clear 1; iIntros "???"; iExists e1, t1; iFrame; eauto 10. }
-  iIntros (Hsteps) "Hσ He Ht". inversion_clear Hsteps as [|?? [t1' σ1']].
+  { inversion_clear 1; iIntros "????"; iExists e1, t1; iFrame; eauto 10. }
+  iIntros (Hsteps) "Hσ He Ht HNC". inversion_clear Hsteps as [|?? [t1' σ1']].
   rewrite -(assoc_L (++)).
-  iMod (wptp_step with "Hσ He Ht") as (e1' t1'' ?) ">H"; first eauto; simplify_eq.
+  iMod (wptp_step with "Hσ He Ht HNC") as (e1' t1'' ?) ">H"; first eauto; simplify_eq.
   iApply (step_fupdN_wand with "H"). iModIntro. iIntros "H".
-  iMod "H" as "(Hσ & He & Ht)". iIntros "!>".
-  by iApply (IH with "Hσ He Ht").
+  iMod "H" as "(Hσ & He & Ht & HNC)". iIntros "!>".
+  by iApply (IH with "Hσ He Ht HNC").
 Qed.
 
 Lemma wpc_safe k κs m e σ Φ Φc :
   state_interp σ κs m -∗
-  WPC e @ k {{ Φ }} {{ Φc }} ={⊤}=∗ ▷^(S (S k))
+  WPC e @ k {{ Φ }} {{ Φc }} -∗ NC ={⊤}=∗ ▷^(S (S k))
   ⌜is_Some (to_val e) ∨ reducible e σ⌝.
 Proof.
-  rewrite wpc_unfold /wpc_pre. iIntros "Hσ (H&_)".
+  rewrite wpc_unfold /wpc_pre. iIntros "Hσ (H&_) HNC".
   destruct (to_val e) as [v|] eqn:?; first by eauto.
-  iSpecialize ("H" $! σ [] κs with "Hσ").
+  iSpecialize ("H" $! σ [] κs with "Hσ HNC").
   iMod (step_fupdN_inner_plain with "[H]") as "H".
   2: { iMod "H". iApply (step_fupdN_wand with "H").
        iModIntro. iIntros "H". iMod "H" as "(H&_)".
@@ -100,25 +105,28 @@ Lemma wptp_strong_adequacy Φ Φc k κs' s n e1 t1 κs t2 σ1 σ2 :
   nsteps n (e1 :: t1, σ1) κs (t2, σ2) →
   state_interp σ1 (κs ++ κs') (length t1) -∗
   WPC e1 @ s; k; ⊤; ∅ {{ Φ }} {{ Φc }} -∗
-  wptp s k t1 -∗ |={⊤,⊤}_(2 * (S (S k)))=>^(S n) (∃ e2 t2',
+  wptp s k t1 -∗
+  NC -∗
+  |={⊤,⊤}_(3 * (S (S k)))=>^(S n) (∃ e2 t2',
     ⌜ t2 = e2 :: t2' ⌝ ∗
     ⌜ ∀ e2, s = NotStuck → e2 ∈ t2 → (is_Some (to_val e2) ∨ reducible e2 σ2) ⌝ ∗
     state_interp σ2 κs' (length t2') ∗
     from_option Φ True (to_val e2) ∗
-    ([∗ list] v ∈ omap to_val t2', fork_post v)).
+    ([∗ list] v ∈ omap to_val t2', fork_post v) ∗
+    NC).
 Proof.
-  iIntros (Hstep) "Hσ He Ht". rewrite Nat_iter_S_r.
-  iDestruct (wptp_steps with "Hσ He Ht") as "Hwp"; first done.
+  iIntros (Hstep) "Hσ He Ht HNC". rewrite Nat_iter_S_r.
+  iDestruct (wptp_steps with "Hσ He Ht HNC") as "Hwp"; first done.
   iApply (step_fupdN_innerN_wand with "Hwp"); auto.
-  iDestruct 1 as (e2' t2' ?) "(Hσ & Hwp & Ht)"; simplify_eq/=.
+  iDestruct 1 as (e2' t2' ?) "(Hσ & Hwp & Ht & HNC)"; simplify_eq/=.
   iMod (fupd_plain_keep_l ⊤
     (▷^(S (S k)) ⌜ ∀ e2, s = NotStuck → e2 ∈ (e2' :: t2') → (is_Some (to_val e2) ∨ reducible e2 σ2) ⌝)%I
-    (state_interp σ2 κs' (length t2') ∗ WPC e2' @ s; k; ⊤; ∅ {{ v, Φ v }} {{ Φc }} ∗ wptp s k t2')%I
-    with "[$Hσ $Hwp $Ht]") as "(Hsafe&Hσ&Hwp&Hvs)".
-  { iIntros "(Hσ & Hwp & Ht)" (e' -> He').
+    (state_interp σ2 κs' (length t2') ∗ WPC e2' @ s; k; ⊤; ∅ {{ v, Φ v }} {{ Φc }} ∗ wptp s k t2' ∗ NC)%I
+    with "[$Hσ $Hwp $Ht $HNC]") as "(Hsafe&Hσ&Hwp&Hvs&HNC)".
+  { iIntros "(Hσ & Hwp & Ht & HNC)" (e' -> He').
     apply elem_of_cons in He' as [<-|(t1''&t2''&->)%elem_of_list_split].
-    - iMod (wpc_safe with "Hσ Hwp") as "$"; auto.
-    - iDestruct "Ht" as "(_ & He' & _)". by iMod (wpc_safe with "Hσ He'"). }
+    - iMod (wpc_safe with "Hσ Hwp HNC") as "$"; auto.
+    - iDestruct "Ht" as "(_ & He' & _)". by iMod (wpc_safe with "Hσ He' HNC"). }
   iApply step_fupd_fupd. iApply step_fupd_intro; first done.
   iMod (fupd_intro_mask' _ ∅) as "Hclo". auto.
   do 5 (iModIntro). iMod "Hclo".
@@ -126,45 +134,48 @@ Proof.
   iApply (step_fupdN_inner_later); auto.
   iNext.
   iExists _, _. iSplitL ""; first done. iFrame "Hsafe Hσ".
-  iSplitL "Hwp".
-  - destruct (to_val e2') as [v2|] eqn:He2'; last done.
-    apply of_to_val in He2' as <-. iApply (wpc_value_inv' with "Hwp").
-  - clear Hstep. iInduction t2' as [|e t2'] "IH"; csimpl; first by iFrame.
-    iDestruct "Hvs" as "[Hv Hvs]". destruct (to_val e) as [v|] eqn:He.
-    + apply of_to_val in He as <-. iMod (wpc_value_inv' with "Hv") as "$".
-      by iApply ("IH" with "[$]").
-    + by iApply ("IH" with "[$]").
+  iMod (wpc_value_inv_option with "Hwp HNC") as "($&HNC)".
+  clear Hstep. iInduction t2' as [|e t2'] "IH"; csimpl; first by iFrame.
+  iDestruct "Hvs" as "[Hv Hvs]". destruct (to_val e) as [v|] eqn:He.
+  + apply of_to_val in He as <-. iMod (wpc_value_inv' with "Hv HNC") as "($&?)".
+    by iApply ("IH" with "[$] [$] [$]").
+  + by iApply ("IH" with "[$] [$] [$]").
 Qed.
 
 Lemma wptp_strong_crash_adequacy Φ Φc κs' s k n e1 t1 κs t2 σ1 σ2 :
   nsteps n (e1 :: t1, σ1) κs (t2, σ2) →
   state_interp σ1 (κs ++ κs') (length t1) -∗
   WPC e1 @ s; k; ⊤; ∅ {{ Φ }} {{ Φc }} -∗
-  wptp s k t1 -∗ |={⊤,⊤}_(2 * S (S k))=>^(S n) |={⊤, ∅}_(S k)=> (∃ e2 t2',
+  wptp s k t1 -∗
+  NC -∗ |={⊤,⊤}_(3 * S (S k))=>^(S n) |={⊤,⊤}_(S k)=> |={⊤, ∅}_(S k)=> (∃ e2 t2',
     ⌜ t2 = e2 :: t2' ⌝ ∗
-    Φc ∗ state_interp σ2 κs' (length t2')).
+    Φc ∗ state_interp σ2 κs' (length t2') ∗ C).
 Proof.
-  iIntros (Hstep) "Hσ He Ht". rewrite Nat_iter_S_r.
-  iDestruct (wptp_steps with "Hσ He Ht") as "Hwp"; first done.
+  iIntros (Hstep) "Hσ He Ht HNC". rewrite Nat_iter_S_r.
+  iDestruct (wptp_steps with "Hσ He Ht HNC") as "Hwp"; first done.
   iApply (step_fupdN_innerN_wand with "Hwp"); auto.
-  iDestruct 1 as (e2' t2' ?) "(Hσ & Hwp & Ht)"; simplify_eq/=.
+  iDestruct 1 as (e2' t2' ?) "(Hσ & Hwp & Ht & HNC)"; simplify_eq/=.
   iMod (fupd_plain_keep_l ⊤
     (▷^(S (S k)) ⌜ ∀ e2, s = NotStuck → e2 ∈ (e2' :: t2') → (is_Some (to_val e2) ∨ reducible e2 σ2) ⌝)%I
-    (state_interp σ2 κs' (length t2') ∗ WPC e2' @ s; k; ⊤; ∅ {{ v, Φ v }} {{ Φc }} ∗ wptp s k t2')%I
-    with "[$Hσ $Hwp $Ht]") as "(Hsafe&Hσ&Hwp&Hvs)".
-  { iIntros "(Hσ & Hwp & Ht)" (e' -> He').
+    (state_interp σ2 κs' (length t2') ∗ WPC e2' @ s; k; ⊤; ∅ {{ v, Φ v }} {{ Φc }} ∗ wptp s k t2' ∗ NC)%I
+    with "[$Hσ $Hwp $Ht $HNC]") as "(Hsafe&Hσ&Hwp&Hvs&HNC)".
+  { iIntros "(Hσ & Hwp & Ht & HNC)" (e' -> He').
     apply elem_of_cons in He' as [<-|(t1''&t2''&->)%elem_of_list_split].
-    - iMod (wpc_safe with "Hσ Hwp") as "$"; auto.
-    - iDestruct "Ht" as "(_ & He' & _)". by iMod (wpc_safe with "Hσ He'"). }
+    - iMod (wpc_safe with "Hσ Hwp HNC") as "$"; auto.
+    - iDestruct "Ht" as "(_ & He' & _)". by iMod (wpc_safe with "Hσ He' HNC"). }
   iApply step_fupd_fupd. iApply step_fupd_intro; first done.
   iMod (fupd_intro_mask' _ ∅) as "Hclo". auto.
   do 5 (iModIntro). iMod "Hclo".
   iApply step_fupdN_inner_fupd.
   iApply (step_fupdN_inner_later); auto.
   iNext. iModIntro.
-  iMod (wpc_crash with "Hwp") as "H".
-  iApply (step_fupdN_inner_wand _ _ (S k) with "H [-]"); eauto.
-  iIntros "($&?)". iExists _, _; eauto.
+  iMod (NC_upd_C with "HNC") as "#HC".
+  iMod (wpc_crash with "Hwp HC") as "H".
+  iModIntro.
+  iApply (step_fupdN_wand _ _ (S k) with "H [-]"); eauto.
+  iIntros "H". iMod "H". iModIntro.
+  iApply (step_fupdN_inner_wand' _ _ _ _ (S k) with "H [-]"); eauto.
+  iIntros "HΦ". iExists _, _; iFrame; eauto.
 Qed.
 End crash_adequacy.
 
@@ -175,29 +186,29 @@ Class pbundleG (T: ofeT) (Σ: gFunctors) := {
 }.
 
 Class perennialG (Λ : language) (CS: crash_semantics Λ) (T: ofeT) (Σ : gFunctors) := PerennialG {
-  perennial_irisG :> ∀ H, pbundleG T Σ → irisG Λ Σ;
+  perennial_irisG :> ∀ (H: invG Σ), pbundleG T Σ → irisG Λ Σ;
   perennial_invG: ∀ H t, @iris_invG _ _ (perennial_irisG H t) = H
 }.
 
 Definition wpr_pre `{perennialG Λ CS T Σ} (s : stuckness) (k: nat)
-    (wpr : invG Σ -d> pbundleG T Σ -d> coPset -d> expr Λ -d> expr Λ -d> (val Λ -d> iPropO Σ) -d>
+    (wpr : invG Σ -d> crashG Σ -d> pbundleG T Σ -d> coPset -d> expr Λ -d> expr Λ -d> (val Λ -d> iPropO Σ) -d>
                      (invG Σ -d> pbundleG T Σ -d> val Λ -d> iPropO Σ) -d> iPropO Σ) :
-  invG Σ -d> pbundleG T Σ -d> coPset -d> expr Λ -d> expr Λ -d> (val Λ -d> iPropO Σ) -d> (invG Σ -d> pbundleG T Σ -d> val Λ -d> iPropO Σ) -d> iPropO Σ :=
-  λ H t E e rec Φ Φr,
+  invG Σ -d> crashG Σ -d> pbundleG T Σ -d> coPset -d> expr Λ -d> expr Λ -d> (val Λ -d> iPropO Σ) -d> (invG Σ -d> pbundleG T Σ -d> val Λ -d> iPropO Σ) -d> iPropO Σ :=
+  λ H1 H2 t E e rec Φ Φr,
   (WPC e @ s ; k; E ; ∅
      {{ Φ }}
      {{ ∀ σ σ' (HC: crash_prim_step CS σ σ') κs n,
-        state_interp σ κs n ={∅}=∗  ▷ ∀ H, ∃ t, state_interp σ' κs 0 ∗ wpr H t E rec rec (λ v, Φr H t v) Φr}})%I.
+        state_interp σ κs n ={∅}=∗  ▷ ∀ H1 H2, NC -∗ ∃ t, state_interp σ' κs 0 ∗ wpr H1 H2 t E rec rec (λ v, Φr H1 t v) Φr ∗ NC}})%I.
 
 Local Instance wpr_pre_contractive `{!perennialG Λ CS T Σ} s k: Contractive (wpr_pre s k).
 Proof.
-  rewrite /wpr_pre=> n wp wp' Hwp ? t E1 e1 rec Φ Φc.
+  rewrite /wpr_pre=> n wp wp' Hwp ?? t E1 e1 rec Φ Φc.
   apply wpc_ne; eauto;
   repeat (f_contractive || f_equiv). apply Hwp.
 Qed.
 
 Definition wpr_def `{!perennialG Λ CS T Σ} (s : stuckness) k :
-  invG Σ → pbundleG T Σ → coPset → expr Λ → expr Λ → (val Λ → iProp Σ) → (invG Σ → pbundleG T Σ → val Λ → iProp Σ) → iProp Σ := fixpoint (wpr_pre s k).
+  invG Σ → crashG Σ → pbundleG T Σ → coPset → expr Λ → expr Λ → (val Λ → iProp Σ) → (invG Σ → pbundleG T Σ → val Λ → iProp Σ) → iProp Σ := fixpoint (wpr_pre s k).
 Definition wpr_aux `{!perennialG Λ CS T Σ} : seal (@wpr_def Λ CS T Σ _). by eexists. Qed.
 Definition wpr `{!perennialG Λ CS T Σ} := wpr_aux.(unseal).
 Definition wpr_eq `{!perennialG Λ CS T Σ} : wpr = @wpr_def Λ CS T Σ _ := wpr_aux.(seal_eq).
@@ -212,48 +223,51 @@ Implicit Types Φc : invG Σ → pbundleG T Σ → val Λ → iProp Σ.
 Implicit Types v : val Λ.
 Implicit Types e : expr Λ.
 
-Lemma wpr_unfold s k Hi t E e rec Φ Φc :
-  wpr s k Hi t E e rec Φ Φc ⊣⊢ wpr_pre s k (wpr s k) Hi t E e rec Φ Φc.
+Lemma wpr_unfold s k Hi Hc t E e rec Φ Φc :
+  wpr s k Hi Hc t E e rec Φ Φc ⊣⊢ wpr_pre s k (wpr s k) Hi Hc t E e rec Φ Φc.
 Proof. rewrite wpr_eq. apply (fixpoint_unfold (wpr_pre s k)). Qed.
 
 (* There's a stronger version of this *)
-Lemma wpr_strong_mono s k Hi t E e rec Φ Ψ Φr Ψr :
-  wpr s k Hi t E e rec Φ Φr -∗
+Lemma wpr_strong_mono s k Hi Hc t E e rec Φ Ψ Φr Ψr :
+  wpr s k Hi Hc t E e rec Φ Φr -∗
   (∀ v, Φ v ==∗ Ψ v) ∧ (∀ Hi t v, Φr Hi t v ==∗ Ψr Hi t v) -∗
-  wpr s k Hi t E e rec Ψ Ψr.
+  wpr s k Hi Hc t E e rec Ψ Ψr.
 Proof.
-  iIntros "H HΦ". iLöb as "IH" forall (e t Hi E Φ Ψ Φr Ψr).
+  iIntros "H HΦ". iLöb as "IH" forall (e t Hi Hc E Φ Ψ Φr Ψr).
   rewrite ?wpr_unfold /wpr_pre.
   iApply (wpc_strong_mono' with "H") ; auto.
   iSplit.
   { iDestruct "HΦ" as "(H&_)". iIntros. iMod ("H" with "[$]"); eauto. }
   iIntros "H".
+  rewrite difference_diag_L.
   iModIntro. iIntros (?????) "Hinterp". iMod ("H" with "[//] Hinterp") as "H".
-  iModIntro. iNext. iIntros (Hi'). iDestruct ("H" $! Hi') as (?) "(?&H)".
+  iModIntro. iNext. iIntros (Hi' Hc') "HNC". iDestruct ("H" $! Hi' Hc' with "[$]") as (?) "(?&H&HNC)".
   iExists _. iFrame. iApply ("IH" with "[$]").
   iSplit; iIntros; iDestruct ("HΦ") as "(_&H)"; by iMod ("H" with "[$]").
 Qed.
 
 (* To prove a recovery wp for e with rec, it suffices to prove a crash wp for e,
    where the crash condition implies the precondition for a crash wp for rec *)
-Lemma idempotence_wpr s k E e rec Φx Φrx Φcx Hi t:
+Lemma idempotence_wpr s k E e rec Φx Φrx Φcx Hi Hc t:
   ((WPC e @ s ; k ; E ; ∅ {{ Φx t }} {{ Φcx t }}) -∗
-   (□ ∀ (H: invG Σ) (t: pbundleG T Σ) σ σ' (HC: crash_prim_step CS σ σ') κs n,
+   (□ ∀ (H: invG Σ) (Hc: crashG Σ) (t: pbundleG T Σ) σ σ' (HC: crash_prim_step CS σ σ') κs n,
         Φcx t -∗ state_interp σ κs n ={∅}=∗
-        ▷ ∀ H', ∃ t', state_interp σ' κs 0 ∗ WPC rec @ s ; k; E ; ∅ {{ Φrx H' t' }} {{ Φcx t' }}) -∗
-    wpr s k Hi t E e rec (Φx t) Φrx)%I.
+        ▷ ∀ H' (Hc': crashG Σ), NC -∗ ∃ t', state_interp σ' κs 0 ∗ WPC rec @ s ; k; E ; ∅ {{ Φrx H' t' }} {{ Φcx t' }} ∗ NC) -∗
+    wpr s k Hi Hc t E e rec (Φx t) Φrx)%I.
 Proof.
-  iLöb as "IH" forall (E e Hi t Φx).
+  iLöb as "IH" forall (E e Hi Hc t Φx).
   iIntros "He #Hidemp".
   rewrite wpr_unfold. rewrite /wpr_pre.
-  iApply (wpc_strong_mono' with "He"); [ auto | auto | auto | ].
-  iSplit; first auto. iIntros "Hcx". iModIntro.
+  iApply (wpc_strong_mono' with "He"); [ auto | auto | auto | set_solver+ | ].
+  iSplit; first auto. iIntros "Hcx".
+  rewrite difference_diag_L.
+  iModIntro.
   iIntros. iMod ("Hidemp" with "[ ] [$] [$]") as "H".
   { eauto. }
-  iModIntro. iNext. iIntros (Hi'). iDestruct ("H" $! Hi') as (t') "(?&Hc)".
+  iModIntro. iNext. iIntros (Hi' Hc') "HNC". iDestruct ("H" $! Hi' Hc' with "[$]") as (t') "(?&Hc&HNC)".
   iExists _. iFrame.
-  iApply ("IH" $! E rec Hi' t' (λ t v, Φrx Hi' t v)%I with "[Hc]").
-  { iApply (wpc_strong_mono' with "Hc"); auto. }
+  iApply ("IH" $! E rec Hi' Hc' t' (λ t v, Φrx Hi' t v)%I with "[Hc]").
+  { iApply (wpc_strong_mono' with "Hc"); rewrite ?difference_diag_L; auto. }
   eauto.
 Qed.
 
@@ -271,39 +285,44 @@ Implicit Types e : expr Λ.
 
 Notation wptp s k t := ([∗ list] ef ∈ t, WPC ef @ s; k; ⊤; ∅ {{ fork_post }} {{ True }})%I.
 
-Fixpoint step_fupdN_fresh k (ns: list nat) Hi0 t0 (P: invG Σ → pbundleG T Σ → iProp Σ) :=
+Fixpoint step_fupdN_fresh k (ns: list nat) Hi0 (Hc0: crashG Σ) t0
+         (P: invG Σ → crashG Σ → pbundleG T Σ → iProp Σ) {struct ns} :=
   match ns with
-  | [] => P Hi0 t0
+  | [] => P Hi0 Hc0 t0
   | (n :: ns) =>
-    (|={⊤, ⊤}_k=>^(S n) |={⊤, ∅}_k=> ▷
-     ∀ Hi', (∃ t' : pbundleG T Σ, step_fupdN_fresh k ns Hi' t' P))%I
+    (|={⊤, ⊤}_k=>^(S (S n)) |={⊤, ∅}_k=> ▷
+     ∀ Hi' Hc', NC -∗ (∃ t' : pbundleG T Σ, step_fupdN_fresh k ns Hi' Hc' t' P))%I
   end.
 
-Lemma step_fupdN_fresh_snoc k (ns: list nat) n Hi0 t0 Q:
-  step_fupdN_fresh k (ns ++ [n]) Hi0 t0 Q ≡
-  step_fupdN_fresh k (ns) Hi0 t0
-    (λ Hi _, |={⊤, ⊤}_k=>^(S n) |={⊤, ∅}_k=> ▷ ∀ Hi', ∃ t', Q Hi' t')%I.
+Lemma step_fupdN_fresh_snoc k (ns: list nat) n Hi0 Hc0 t0 Q:
+  step_fupdN_fresh k (ns ++ [n]) Hi0 Hc0 t0 Q ≡
+  step_fupdN_fresh k (ns) Hi0 Hc0 t0
+    (λ Hi Hc' _, |={⊤, ⊤}_k=>^(S (S n)) |={⊤, ∅}_k=> ▷ ∀ Hi' Hc', NC -∗ ∃ t', Q Hi' Hc' t')%I.
 Proof.
   apply (anti_symm (⊢)%I).
-  - revert Hi0 t0 Q.
-    induction ns => ??? //=. do 1 f_equiv.
-    apply step_fupdN_mono. apply fupd_mono.
+  - revert Hi0 Hc0 t0 Q.
+    induction ns => ????; first by auto.
     iIntros "H".
-    iApply (step_fupdN_innerN_wand with "H"); auto.
+    iApply (step_fupdN_innerN_wand ⊤ ⊤ k k with "[H] []"); auto.
     iIntros "H".
     iApply (step_fupdN_inner_wand' with "H"); auto.
-    iIntros "H". iNext. iIntros.
-    iDestruct ("H" $! _) as (?) "H".
+    iIntros "H".
+    iNext. iIntros (??) "HNC".
+    iDestruct ("H" $! _ _ with "[$]") as (?) "H".
     iExists _. by iApply IHns.
-  - revert Hi0 t0 Q.
-    induction ns => ??? //=. do 1 f_equiv.
+  - revert Hi0 Hc0 t0 Q.
+    induction ns => ???? //=.
+    do 1 f_equiv.
     apply step_fupdN_mono. apply fupd_mono.
+    iIntros "H".
+    iApply (step_fupdN_inner_wand with "H"); auto.
     iIntros "H".
     iApply (step_fupdN_innerN_wand with "H"); auto.
     iIntros "H".
     iApply (step_fupdN_inner_wand' with "H"); auto.
-    iIntros "H". iNext. iIntros.
-    iDestruct ("H" $! _) as (?) "H".
+    iIntros "H".
+    iNext. iIntros (??) "HNC".
+    iDestruct ("H" $! _ _ with "[$]") as (?) "H".
     iExists _. by iApply IHns.
 Qed.
 
@@ -349,37 +368,38 @@ Proof.
   iNext. rewrite -laterN_later => //=.
 Qed.
 
-Lemma step_fupdN_fresh_wand k (ns: list nat) Hi0 t0 Q Q':
-  step_fupdN_fresh k (ns) Hi0 t0 Q -∗ (∀ Hinv t, Q Hinv t -∗ Q' Hinv t)
-  -∗ step_fupdN_fresh k ns Hi0 t0 Q'.
+Lemma step_fupdN_fresh_wand k (ns: list nat) Hi0 Hc0 t0 Q Q':
+  step_fupdN_fresh k (ns) Hi0 Hc0 t0 Q -∗ (∀ Hinv Hc t, Q Hinv Hc t -∗ Q' Hinv Hc t)
+  -∗ step_fupdN_fresh k ns Hi0 Hc0 t0 Q'.
 Proof.
-  revert Hi0 t0.
-  induction ns => ??.
+  revert Hi0 Hc0 t0.
+  induction ns => ???.
   - iIntros "H Hwand". iApply "Hwand". eauto.
-  - iIntros "H Hwand". simpl.
+  - iIntros "H Hwand". rewrite /step_fupdN_fresh -/step_fupdN_fresh.
     iApply (step_fupdN_fresh_pattern_wand with "H [Hwand]").
     iIntros "H".
-    iIntros (Hi'). iSpecialize ("H" $! Hi'). iDestruct "H" as (?) "H".
+    iIntros (Hi' Hc') "HNC". iSpecialize ("H" $! Hi' Hc' with "[$]"). iDestruct "H" as (?) "H".
     iExists _. iApply (IHns with "H"). eauto.
 Qed.
 
 Fixpoint fresh_later_count k (ns: list nat) :=
   match ns with
   | [] => (S (S k))
-  | n :: ns' => (S (S n) * (S (S k))) + fresh_later_count k ns'
+  | n :: ns' => (S (S (S n)) * (S (S k))) + fresh_later_count k ns'
   end.
 
-Lemma step_fupdN_fresh_plain `{!invPreG Σ} P `{!Plain P} k ns n:
-  (∀ Hinv', |={⊤}=> ∃ t, step_fupdN_fresh k ns Hinv' t
-                  (λ _ _, |={⊤, ⊤}_k=>^(S n) |={⊤, ∅}=> P)) -∗
-  ▷^(fresh_later_count k ns + S (S k + n * (S (S k)))) P.
+Lemma step_fupdN_fresh_plain `{!invPreG Σ} `{!crashPreG Σ} P `{!Plain P} k ns n:
+  (∀ Hinv' Hc', NC -∗ |={⊤}=> ∃ t, step_fupdN_fresh k ns Hinv' Hc' t
+                  (λ _ _ _, |={⊤, ⊤}_k=>^(S n) |={⊤, ∅}=> P)) -∗
+  ▷^(fresh_later_count k ns + S (S k + S n * (S (S k)))) P.
 Proof.
   iIntros "H".
   iInduction ns as [| n' ns] "IH".
   - rewrite /step_fupdN_fresh.
     iApply (bupd_plain (▷^(_) P)%I); try (iPureIntro; apply _).
     iMod wsat_alloc as (Hinv) "(Hw&HE)".
-    iSpecialize ("H" $! Hinv).
+    iMod NC_alloc as (Hc) "HNC".
+    iSpecialize ("H" $! Hinv Hc with "HNC").
     rewrite {1}uPred_fupd_eq {1}/uPred_fupd_def.
     iMod ("H" with "[$]") as "[>Hw [>HE >H]]".
     iDestruct ("H") as (_) "H".
@@ -389,15 +409,16 @@ Proof.
     rewrite {1}uPred_fupd_eq {1}/uPred_fupd_def.
     iMod ("H" with "[$]") as "[Hw [HE >$]]"; eauto.
   - iMod wsat_alloc as (Hinv) "(Hw&HE)".
+    iMod NC_alloc as (Hc) "HNC".
     iSpecialize ("H" $! Hinv).
     rewrite {1}uPred_fupd_eq {1}/uPred_fupd_def.
-    iMod ("H" with "[$]") as "[>Hw [>HE >H]]".
+    iMod ("H" with "HNC [$]") as "[>Hw [>HE >H]]".
     iDestruct "H" as (t) "H".
     rewrite /step_fupdN_fresh -/step_fupdN_fresh.
     iDestruct (step_fupdN_fresh_pattern_wand  _ _ _
                   (▷^(fresh_later_count k ns + _) P)
                  with "H [IH]") as "H".
-    { iIntros "H". iApply "IH". iIntros. iModIntro. iApply "H". }
+    { iIntros "H". iApply "IH". iIntros. iModIntro. by iApply "H". }
     iDestruct (step_fupdN_fresh_pattern_plain' with "H") as "H".
     rewrite {1}uPred_fupd_eq {1}/uPred_fupd_def.
     iMod ("H" with "[$]") as "[Hw [HE >H]]".
@@ -405,15 +426,15 @@ Proof.
 Qed.
 
 (* XXX this probably needs to be tweaked. *)
-Lemma step_fupdN_fresh_soundness `{!invPreG Σ} (φ : Prop) k ns n:
-  (∀ Hinv : invG Σ, (|={⊤}=> (∃ t0, step_fupdN_fresh k ns Hinv t0
-                             (λ _ _, |={⊤, ⊤}_k=>^(S n) |={⊤, ∅}=> ▷ ⌜φ⌝)))%I) →
+Lemma step_fupdN_fresh_soundness `{!invPreG Σ} `{!crashPreG Σ} (φ : Prop) k ns n:
+  (∀ (Hinv : invG Σ) (Hc: crashG Σ), NC -∗ (|={⊤}=> (∃ t0, step_fupdN_fresh k ns Hinv Hc t0
+                             (λ _ _ _, |={⊤, ⊤}_k=>^(S (S n)) |={⊤, ∅}=> ▷ ⌜φ⌝)))%I) →
   φ.
 Proof.
   intros Hiter.
   eapply (soundness (M:=iResUR Σ) _  (fresh_later_count k ns + _ + 1)); simpl.
   rewrite laterN_plus.
-  iApply step_fupdN_fresh_plain. iIntros (Hinv). iApply Hiter.
+  iApply step_fupdN_fresh_plain. iIntros (Hinv Hc). iApply Hiter.
 Qed.
 
 (*
@@ -423,22 +444,23 @@ Notation "P ={ E }=∗_ t Q" := (P -∗ |={E}=>_(t) Q)%I
  (at level 99) : bi_scope.
 *)
 
-Lemma wptp_recv_strong_normal_adequacy Φ Φr κs' s k Hi t n ns r1 e1 t1 κs t2 σ1 σ2 :
+Lemma wptp_recv_strong_normal_adequacy Φ Φr κs' s k Hi Hc t n ns r1 e1 t1 κs t2 σ1 σ2 :
   nrsteps (CS := CS) r1 (ns ++ [n]) (e1 :: t1, σ1) κs (t2, σ2) Normal →
   state_interp σ1 (κs ++ κs') (length t1) -∗
-  wpr s k Hi t ⊤ e1 r1 Φ Φr -∗
-  wptp s k t1 -∗ step_fupdN_fresh (2 * (S (S k))) ns Hi t (λ Hi' t',
-    ⌜ Hi' = Hi ∧ t' = t ⌝ ∗
-    (|={⊤, ⊤}_(2 * (S (S k)))=>^(S n) |={⊤, ∅}=> ▷ ∃ e2 t2',
+  wpr s k Hi Hc t ⊤ e1 r1 Φ Φr -∗
+  wptp s k t1 -∗ NC -∗ step_fupdN_fresh (3 * (S (S k))) ns Hi Hc t (λ Hi' Hc' t',
+    ⌜ Hi' = Hi ∧ Hc' = Hc ∧ t' = t ⌝ ∗
+    (|={⊤, ⊤}_(3 * (S (S k)))=>^(S n) |={⊤, ∅}=> ▷ ∃ e2 t2',
     ⌜ t2 = e2 :: t2' ⌝ ∗
     ⌜ ∀ e2, s = NotStuck → e2 ∈ t2 → (is_Some (to_val e2) ∨ reducible e2 σ2) ⌝ ∗
     state_interp σ2 κs' (length t2') ∗
     from_option Φ True (to_val e2) ∗
-    ([∗ list] v ∈ omap to_val t2', fork_post v))).
+    ([∗ list] v ∈ omap to_val t2', fork_post v) ∗
+    NC)).
 Proof.
-  iIntros (Hstep) "Hσ He Ht".
+  iIntros (Hstep) "Hσ He Ht HNC".
   inversion Hstep. subst.
-  iPoseProof (wptp_strong_adequacy with "Hσ [He] Ht") as "H".
+  iPoseProof (wptp_strong_adequacy with "Hσ [He] Ht HNC") as "H".
   { eauto. }
   {rewrite wpr_unfold /wpr_pre. iApply "He". }
   assert (ns = []) as ->;
@@ -452,34 +474,41 @@ Proof.
   iNext. eauto.
 Qed.
 
-Lemma wptp_recv_strong_crash_adequacy Φ Φr κs' s k Hi t ns n r1 e1 t1 κs t2 σ1 σ2 :
+Lemma wptp_recv_strong_crash_adequacy Φ Φr κs' s k Hi Hc t ns n r1 e1 t1 κs t2 σ1 σ2 :
   nrsteps (CS := CS) r1 (ns ++ [n]) (e1 :: t1, σ1) κs (t2, σ2) Crashed →
   state_interp σ1 (κs ++ κs') (length t1) -∗
-  wpr s k Hi t ⊤ e1 r1 Φ Φr -∗
-  wptp s k t1 -∗ step_fupdN_fresh (2 * (S (S k))) ns Hi t (λ Hi' t',
-    (|={⊤, ⊤}_(2 * (S (S k)))=>^(S n) |={⊤, ∅}=> ▷ ∃ e2 t2',
+  wpr s k Hi Hc t ⊤ e1 r1 Φ Φr -∗
+  wptp s k t1 -∗ NC -∗ step_fupdN_fresh (3 * (S (S k))) ns Hi Hc t (λ Hi' Hc' t',
+    (|={⊤, ⊤}_(3 * (S (S k)))=>^(S (S n)) |={⊤, ∅}=> ▷ ∃ e2 t2',
     ⌜ t2 = e2 :: t2' ⌝ ∗
     ⌜ ∀ e2, s = NotStuck → e2 ∈ t2 → (is_Some (to_val e2) ∨ reducible e2 σ2) ⌝ ∗
     state_interp σ2 κs' (length t2') ∗
     from_option (Φr Hi' t') True (to_val e2) ∗
-    ([∗ list] v ∈ omap to_val t2', fork_post v))).
+    ([∗ list] v ∈ omap to_val t2', fork_post v) ∗
+    NC)).
 Proof.
-  revert Hi t e1 t1 κs κs' t2 σ1 σ2 Φ.
-  induction ns as [|n' ns' IH] => Hi t e1 t1 κs κs' t2 σ1 σ2 Φ.
+  revert Hi Hc t e1 t1 κs κs' t2 σ1 σ2 Φ.
+  induction ns as [|n' ns' IH] => Hi Hc t e1 t1 κs κs' t2 σ1 σ2 Φ.
   { rewrite app_nil_l.
     inversion 1.
     match goal with
     | [ H : nrsteps _ _ _ _ _ _ |- _ ] => inversion H
     end.
   }
-  iIntros (Hsteps) "Hσ He Ht".
+  iIntros (Hsteps) "Hσ He Ht HNC".
   inversion_clear Hsteps as [|?? [t1' σ1'] ????? s0].
   rewrite {1}/step_fupdN_fresh -/step_fupdN_fresh.
   destruct ρ2 as (?&σ2_pre_crash).
   iApply (step_fupdN_innerN_wand with "[-]"); try reflexivity.
   { rewrite -assoc wpr_unfold /wpr_pre.
-    iPoseProof (@wptp_strong_crash_adequacy with "[$] [$]") as "H"; eauto.
-    rewrite perennial_invG. by iApply "H".
+    iPoseProof (@wptp_strong_crash_adequacy with "[$] [$] [$] [$]") as "H"; eauto.
+    iEval (rewrite Nat_iter_S_r).
+    rewrite perennial_invG.
+    iApply (step_fupdN_innerN_wand ⊤ ⊤ (3 * (S (S k))) _ (S n') (S n') with "H"); auto.
+    iIntros "H".
+    iApply (step_fupdN_inner_wand with "H"); auto.
+    { lia. }
+    iIntros "H". iApply "H".
   }
   iIntros "H".
   rewrite -step_fupdN_inner_fupd.
@@ -488,28 +517,29 @@ Proof.
   { reflexivity. }
   { lia. }
   iIntros "H".
-  iDestruct "H" as (e2 t2' ?) "(H&Hσ)".
+  iDestruct "H" as (e2 t2' ?) "(H&Hσ&HC)".
   iMod ("H" with "[//] Hσ") as "H". iModIntro. iNext.
   destruct s0.
-  - iIntros (Hi'). iSpecialize ("H" $! Hi').
-    iDestruct "H" as (t') "(Hσ&Hr)".
-    iPoseProof (IH with "[Hσ] Hr []") as "H"; eauto.
-  - iIntros (Hi').
-    iDestruct ("H" $! Hi') as (t') "(Hσ&Hr)".
+  - iIntros (Hi' Hc') "HNC". iSpecialize ("H" $! Hi' Hc' with "[$]").
+    iDestruct "H" as (t') "(Hσ&Hr&HNC)".
+    iPoseProof (IH with "[Hσ] Hr [] HNC") as "H"; eauto.
+  - iIntros (Hi' Hc') "HNC".
+    iDestruct ("H" $! Hi' Hc' with "[$]") as (t') "(Hσ&Hr&HNC)".
     iExists t'.
-    iDestruct (wptp_recv_strong_normal_adequacy with "[Hσ] [Hr] []") as "H"; eauto.
+    iDestruct (wptp_recv_strong_normal_adequacy with "[Hσ] [Hr] [] HNC") as "H"; eauto.
     iApply (step_fupdN_fresh_wand with "H").
-    iIntros (??) "H".
-    iDestruct "H" as ((?&?)) "H". subst.
-    iApply "H".
+    iIntros (???) "H".
+    iDestruct "H" as ((?&?&?)) "H". subst.
+    iClear "HC".
+    iApply (step_fupdN_innerN_wand with "H"); auto.
 Qed.
 
-Lemma wptp_recv_strong_adequacy Φ Φr κs' s k Hi t ns n r1 e1 t1 κs t2 σ1 σ2 stat :
+Lemma wptp_recv_strong_adequacy Φ Φr κs' s k Hi Hc t ns n r1 e1 t1 κs t2 σ1 σ2 stat :
   nrsteps (CS := CS) r1 (ns ++ [n]) (e1 :: t1, σ1) κs (t2, σ2) stat →
   state_interp σ1 (κs ++ κs') (length t1) -∗
-  wpr s k Hi t ⊤ e1 r1 Φ Φr -∗
-  wptp s k t1 -∗ step_fupdN_fresh (2 * (S (S k))) ns Hi t (λ Hi' t',
-    (|={⊤, ⊤}_(2 * (S (S k)))=>^(S n) |={⊤, ∅}=> ▷ ∃ e2 t2',
+  wpr s k Hi Hc t ⊤ e1 r1 Φ Φr -∗
+  wptp s k t1 -∗ NC -∗ step_fupdN_fresh (3 * (S (S k))) ns Hi Hc t (λ Hi' Hc' t',
+    (|={⊤, ⊤}_(3 * (S (S k)))=>^(S (S n)) |={⊤, ∅}=> ▷ ∃ e2 t2',
     ⌜ t2 = e2 :: t2' ⌝ ∗
     ⌜ ∀ e2, s = NotStuck → e2 ∈ t2 → (is_Some (to_val e2) ∨ reducible e2 σ2) ⌝ ∗
     state_interp σ2 κs' (length t2') ∗
@@ -517,14 +547,15 @@ Lemma wptp_recv_strong_adequacy Φ Φr κs' s k Hi t ns n r1 e1 t1 κs t2 σ1 σ
      | Normal => ⌜ Hi' = Hi ∧ t' = t ⌝ ∗ from_option Φ True (to_val e2)
      | Crashed => from_option (Φr Hi' t') True (to_val e2)
      end)  ∗
-    ([∗ list] v ∈ omap to_val t2', fork_post v))).
+    ([∗ list] v ∈ omap to_val t2', fork_post v) ∗
+    NC)).
 Proof.
   intros. destruct stat.
   - by iApply wptp_recv_strong_crash_adequacy.
-  - iIntros. iDestruct (wptp_recv_strong_normal_adequacy with "[$] [$] [$]") as "H"; eauto.
+  - iIntros. iDestruct (wptp_recv_strong_normal_adequacy with "[$] [$] [$] [$]") as "H"; eauto.
     iApply (step_fupdN_fresh_wand with "H").
-    iIntros (??) "H".
-    iDestruct "H" as ((?&?)) "H". subst.
+    iIntros (???) "H".
+    iDestruct "H" as ((?&?&?)) "H". subst.
     iApply (step_fupdN_innerN_wand with "H"); auto.
     iIntros ">H !> !> ".
     iDestruct "H" as (????) "(H&?&?)". iExists _, _.
@@ -562,8 +593,8 @@ Proof.
   - constructor; naive_solver.
 Qed.
 
-Corollary wp_recv_adequacy Σ Λ CS (T: ofeT) `{!invPreG Σ} s k e r σ φ φr :
-  (∀ `{Hinv : !invG Σ} κs,
+Corollary wp_recv_adequacy Σ Λ CS (T: ofeT) `{!invPreG Σ} `{!crashPreG Σ} s k e r σ φ φr :
+  (∀ `{Hinv : !invG Σ} `{Hc: !crashG Σ} κs,
      (|={⊤}=> ∃ (t: pbundleG T Σ)
          (stateI : pbundleG T Σ→ state Λ → list (observation Λ) → iProp Σ)
          (fork_post : pbundleG T Σ → val Λ → iProp Σ) Hpf,
@@ -573,25 +604,26 @@ Corollary wp_recv_adequacy Σ Λ CS (T: ofeT) `{!invPreG Σ} s k e r σ φ φr :
                IrisG Λ Σ Hi (λ σ κs _, stateI t σ κs)
                     (fork_post t)) Hpf
                in
-       stateI t σ κs ∗ wpr s k Hinv t ⊤ e r (λ v, ⌜φ v⌝) (λ _ _ v, ⌜φr v⌝))%I) →
+       stateI t σ κs ∗ wpr s k Hinv Hc t ⊤ e r (λ v, ⌜φ v⌝) (λ _ _ v, ⌜φr v⌝))%I) →
   recv_adequate (CS := CS) s e r σ (λ v _, φ v) (λ v _, φr v) .
 Proof.
   intros Hwp.
   apply recv_adequate_alt.
   intros t2 σ2 stat [n [κs H]]%erased_rsteps_nrsteps.
   destruct (nrsteps_snoc _ _ _ _ _ _ H) as (ns'&n'&->).
-  eapply (step_fupdN_fresh_soundness _ (2 * (S (S k))) ns' n')=> Hinv.
-  iMod (Hwp Hinv κs) as (t stateI Hfork_post Hpf) "(Hw&H)".
+  eapply (step_fupdN_fresh_soundness _ (3 * (S (S k))) ns' n')=> Hinv Hc.
+  iIntros "HNC".
+  iMod (Hwp Hinv Hc κs) as (t stateI Hfork_post Hpf) "(Hw&H)".
   iModIntro. iExists _.
   iDestruct (wptp_recv_strong_adequacy
                (perennialG0 :=
           PerennialG _ _ T Σ
             (λ Hi t,
              IrisG Λ Σ Hi (λ σ κs _, stateI t σ κs)
-                  (Hfork_post t)) Hpf) _ _ [] with "[Hw] [H] []") as "H"; eauto.
+                  (Hfork_post t)) Hpf) _ _ [] with "[Hw] [H] [] HNC") as "H"; eauto.
   { rewrite app_nil_r. eauto. }
   iApply (step_fupdN_fresh_wand with "H").
-  iIntros (??) "H".
+  iIntros (???) "H".
   iApply (step_fupdN_innerN_wand with "H"); auto.
   iIntros ">H !> !> ".
   iDestruct "H" as (v2 ???) "(_&Hv&Hnstuck)".
