src/program_logic/staged_invariant.v
@@ -13,6 +13,13 @@ Definition NC_tok : crashR := Cinl (Excl ()).
 Definition C_tok : crashR := Cinr (to_agree ()).
 
 Class crashG Σ := { crash_inG :> inG Σ crashR; crash_name : gname }.
+Class crashPreG Σ := { crash_inPreG :> inG Σ crashR }.
+
+Definition crashΣ : gFunctors :=
+    #[GFunctor (csumR (exclR unitO) (agreeR unitO))].
+
+Instance subG_crashG {Σ} : subG crashΣ Σ → crashPreG Σ.
+Proof. solve_inG. Qed.
 
 Definition NC_def `{crashG Σ} := own crash_name NC_tok.
 Definition NC_aux `{crashG Σ} : seal NC_def. by eexists. Qed.
@@ -21,6 +28,14 @@ Definition C_def `{crashG Σ} := own crash_name C_tok.
 Definition C_aux `{crashG Σ} : seal C_def. by eexists. Qed.
 Definition C `{crashG Σ} := C_aux.(unseal).
 
+Lemma NC_alloc `{!crashPreG Σ} : (|==> ∃ _ : crashG Σ, NC)%I.
+Proof.
+  iIntros.
+  iMod (own_alloc (Cinl (Excl ()))) as (γ) "H".
+  { econstructor. }
+  iExists {| crash_name := γ |}.
+  rewrite /NC NC_aux.(seal_eq). by iFrame.
+Qed.
 
 Class stagedG (Σ : gFunctors) : Set := WsatG {
   staging_saved_inG :> savedPropG Σ;
@@ -58,6 +73,23 @@ Proof. rewrite /C C_aux.(seal_eq). apply _. Qed.
 
 Global Instance NC_timeless : Timeless NC.
 Proof. rewrite /NC NC_aux.(seal_eq). apply _. Qed.
+
+Lemma NC_C: NC -∗ C -∗ False.
+Proof.
+ rewrite /C C_aux.(seal_eq).
+ rewrite /NC NC_aux.(seal_eq).
+  iIntros "H H'".
+  { by iDestruct (own_valid_2 with "H H'") as %?. }
+Qed.
+
+Lemma NC_upd_C: NC ==∗ C.
+Proof.
+ rewrite /C C_aux.(seal_eq).
+ rewrite /NC NC_aux.(seal_eq).
+ iIntros "H". iMod (own_update with "H") as "$".
+ { by apply cmra_update_exclusive. }
+ done.
+Qed.
 
 Global Instance staged_contractive N k E E' γ γ' : Contractive (staged_inv N k E E' γ γ').
 Proof.
